---
layout: post
title: Davidson and MacKinnon Chapter 2&mdash;The Geometry of Linear Regression
date: 2022-10-23 11:12:00-0400
description: The second chapter of Econometric Theory and Methods
tags: note econometics
categories: 
---

# Introduction

A linear regression model with $$k$$ regressors 

$$\label{eq1}
\mathbf{y}=\mathbf{X}\beta+\mathbf{u}$$

where $$y$$ and $$u$$
are $$n-$$vectors, $$X$$ is an $$n\times k$$ matrix, and $$\beta$$ is
a $$k-$$vector.

$$\begin{eqnarray}
\label{eq2}
y&=&\left[\begin{array}{c}
y_{1}\\
y_{2}\\
\vdots\\
y_{n}
\end{array}
\right],
\beta=\left[\begin{array}{c}
\beta_{1}\\
\beta_{2}\\
\vdots\\
\beta_{k}
\end{array}
\right],
u=\left[\begin{array}{c}
u_{1}\\
u_{2}\\
\vdots\\
u_{n}
\end{array}
\right],
\end{eqnarray}$$

$$\begin{eqnarray}
\label{eq3}
X&=&\left[\begin{array}{cccc}
X_{11}&X_{12}&\cdots&X_{1k}\\
X_{21}&X_{22}&\cdots&X_{2k}\\
\vdots&\vdots&&\vdots\\
X_{n1}&X_{n2}&\cdots&X_{nk}
\end{array}
\right]
\end{eqnarray}$$

A typical row of this equation is 

$$\begin{eqnarray}
\label{eq4}
y_{t}&=&X_{t}\beta+u_{t}=\sum_{i=1}^{k}\beta_{i}X_{ti}+u_{t}
\end{eqnarray}$$ 

where $$X_{t}$$ denotes the $$t^{th}$$ row of $$X$$
OLS estimates of the vector $$\beta$$ are $$\label{eq5}
\hat{\beta}=(X^{T}X)^{-1}X^{T}y$$

-   **numerical properties:** properties of estimates if they have
    nothing to do with how the data were actually generated. Such
    properties hold for every set of data by virtue of the way in which
    $$\hat{\beta}$$ is computed, and the fact that they hold can
    always be verified by direct calculation.

-   **statistical properties:** depend on unverifiable assumptions about
    how the data were generated, and they can never be verified for any
    actual data set.

# The Geometry of OLS Estimation

We partition $$X$$ in terms of its columns as follows,

$$\begin{eqnarray}
X&=&\left[\begin{array}{cccc}
x_{1}&x_{2}&\cdots&x_{k}
\end{array}
\right]
\end{eqnarray}$$ is just a linear combination of the columns of $$X$$.

Then we find that $$\begin{eqnarray}
\bm{X\beta}&=&\left[\begin{array}{cccc}
x_{1}&x_{2}&\cdots&x_{k}
\end{array}
\right]\left[\begin{array}{c}
\beta_{1}\\
\beta_{2}\\
\vdots\\
\beta_{k}
\end{array}
\right]\\
&=&x_{1}\beta_{1}+x_{2}\beta_{2}+\dots+x_{k}\beta_{k}=\sum_{i=1}^{k}\beta_{i}x_{i}
\end{eqnarray}$$

Any $$n$$-vector $$\bm{X\beta}$$ belongs to $$S(x)$$, which is a
$$k$$-dimensional subspace of $$E^{n}$$. In particular, the vector
$$\bm{X\hat{\beta}}$$ constructed using the OLS estimator
$$\bm{\hat{\beta}}$$ belongs to this subspace.

The estimator $$\bm{\hat{\beta}}$$ was obtained by solving the equation (\ref{eqp8}).

$$\begin{eqnarray}
\label{eqp8}
X^{T}(y-\bm{X\hat{\beta}})&=&\bm{0}
\end{eqnarray}$$

We select a single row of matrix product in (\ref{eqp8}), the $$i^{th}$$
element is 

$$\begin{eqnarray}
\label{eqp9}
x^{T}_{i}(y-\bm{X\hat{\beta}})&=&\langlex^{T}_{i},y-\bm{X\hat{\beta}}\rangle=0
\end{eqnarray}$$

(\ref{eqp9}) means that
the vector $$y-\bm{X\hat{\beta}}$$ is orthogonal to all of the
regressors $$x_{i}$$. As a result, (\ref{eqp8}) is referred to as **orthogonality conditions**

(\ref{eqp9}) also means
that $$\bm{\hat{u}}$$ is orthogonal to all the regressors, which implies
that $$\bm{\hat{u}}$$ is orthogonal to every vector in $$S(X)$$, the
span of the regressors.

The vector $$\bm{X\hat{\beta}}$$ is referred to as the vector of **fitted
values**, and it lies in $$S(X)$$. Consequently, $$\bm{X\hat{\beta}}$$
must be orthogonal to $$\bm{\hat{u}}$$.

From Figure [\[fig:1\]](#fig:1){reference-type="ref" reference="fig:1"}
we observe that the shortest distance from $$y$$ to the horizontal
plane is obtained by descending vertically on to it, and the point in
the horizontal plane vertically below $$y$$ , labeled $$A$$ in the
figure, is the closest point in the plane to $$y$$. Thus
$$\|\bm{\hat{u}}\|$$ minimizes $$\|\bm{u(\beta)}\|$$.

We can see that $$y$$ is the hypotenuse of the triangle, the other
two sides being $$\bm{X\hat{\beta}}$$ and $$\bm{\hat{u}}$$. We have

$$\begin{eqnarray}
\label{eqp10}
\|y\|^{2}&=&\|\bm{X\hat{\beta}}\|^{2}+\|\bm{\hat{u}}\|^{2}
\end{eqnarray}$$

We can rerwrite it as scalar products 

$$\begin{eqnarray}
\label{eqp11}
y^{T}y&=&\bm{\hat{\beta}}^{T}X^{T}X\bm{\hat{\beta}}+(y-\bm{X\hat{\beta}})^{T}(y-\bm{X\hat{\beta}})
\end{eqnarray}$$ The **total sum of squares(TSS)** is equal to the
**explained sum of squares(ESS)** plus the **sum of squared
residuals(SSR)**

## Orthogonal Projections

When we estimate a linear regression model, we map the regressand
$$y$$ into a vector of fitted $$\bm{X\hat{\beta}}$$ and a vector of
residuals $$\bm{\hat{u}}=y-\bm{X\hat{\beta}}$$. These mappings are
examples of orthogonal projections.

A **projection** is a mapping that takes each point of $$E^{n}$$ into a
point in a subspace of $$E^{n}$$, while leaving all points in that
subspace unchanged. An **orthogonal projection** maps any point into the
point of the subspace that is closest to it.

An orthogonal projection on to a given subspace can be performed by
premultiplying the vector to be projected by a suitable **projection
matrix**. In OLS, we use the following two projections matrices that
yield the vector of fitted values and the vector of residuals

$$\begin{eqnarray}
\label{eqp12}
\bm{P_{X}}&=&X\left(X^{T}X\right)^{-1}X^{T}\\
\nonumber
\bm{M_{X}}&=&\bm{I-P_{X}}=\bm{I}-X\left(X^{T}X\right)^{-1}X^{T}
\end{eqnarray}$$

Properties

1.  $$\begin{eqnarray}
    \label{eqp13}
    X\hat{\beta}&=&X(X^{T}X)^{-1}X^{T}y=P_{X}y\\\nonumber
    \hat{u}&=&y-X\hat{\beta}=(I-P_{X})y=M_{X}y
    \end{eqnarray}$$ 

    (\ref{eqp13}) says that projection matrix $$\bm{P_{X}}$$
    projects on to $$S(X)$$. For any $$n-$$vector $$y$$,
    $$\bm{P_{X}y}$$ always lies in $$S(X)$$.

    The **image** of $$\bm{P_{X}}$$, which is a shorter name for its
    invariant subspace, is precisely $$S(X)$$. The image of
    $$\bm{M_{X}}$$ is $$S^{\bot}(X)$$, the orthogonal complement of
    image of $$\bm{P_{X}}$$.

2.  Symmetric and idempotent 

$$\begin{eqnarray}
    \bm{P}_{X}^{T}&=&\bm{P}_{X}\\
    \bm{P}_{X}\bm{P}_{X}&=&\bm{P}_{X}\\
    \bm{M}_{X}^{T}&=&\bm{M}_{X}\\
    \bm{M}_{X}\bm{M}_{X}&=&\bm{M}_{X}
    \end{eqnarray}$$ 

    We can think that project a vector it on to
    $$S(X)$$, and then project it on to $$S(X)$$ again, the second
    projection has no effect at all. So it is left unchanged. For any
    vector $$y$$, we have 

    $$\begin{eqnarray}
    \label{eqp17}
    P_{X}P_{X}y&=&P_{X}y
    \end{eqnarray}$$

3.  $$\begin{eqnarray}
    \bm{P_{X}X}&=&X\\
    \bm{M_{X}X}&=&\bm{0}
    \end{eqnarray}$$

4.  $$\bm{P_{X}}$$ and $$\bm{M_{X}}$$ annihilate each other

    $$\begin{eqnarray}
    \label{eqp19}
    \bm{P_{X}}\bm{M_{X}}&=&\bm{0}
    \end{eqnarray}$$ 

    The projection matrix $$\bm{M_{X}}$$ annihilates all
    points that lie in $$S(X)$$, and $$\bm{P_{X}}$$ likewise
    annihilates all points that lie in $$S^{\bot}(X)$$.

5.  $$X=\left[\begin{array}{cc}
    x_{1}&x_{2}
    \end{array}\right]$$

    $$\begin{eqnarray}
    \bm{P_{x_{1}}}&=&\bm{P_{X}}\\
    \bm{P_{x_{1}}}\bm{P_{X}}&=&\bm{P_{X}}\bm{P_{x_{1}}}=\bm{P_{x_{1}}}\\
    \bm{M_{x_{1}}}&=&\bm{M_{X}}\\
    \bm{M_{x_{1}}}\bm{M_{X}}&=&\bm{M_{X}}\bm{M_{x_{1}}}=\bm{M_{X}}
    \end{eqnarray}$$

6.  Pythagoras' Theorem 

$$\begin{eqnarray}
    \norm{y}^{2}&=&\norm{\bm{P_{X}y}}^{2}+\norm{\bm{M_{X}y}}^{2}
    \end{eqnarray}$$

## Linear Transformations of Regressors

If $$\bm{A}$$ is any nonsingular $$k\times k$$ matrix, we postmultiply
$$X$$ by $$\bm{A}$$. It is called a **nonsingular linear
transformation** 

$$\begin{eqnarray}
\bm{XA}&=&X\left[\begin{array}{cccc}
\bm{a}_{1}&\bm{a}_{2}&\cdots&\bm{a}_{k}
\end{array}\right]\\
&=&\left[\begin{array}{cccc}
X\bm{a}_{1}&X\bm{a}_{2}&\cdots&X\bm{a}_{k}
\end{array}\right]
\end{eqnarray}$$

where $$\bm{Xa}_{i}$$ is an $$n-$$vector that is a linear combination of
columns of $$X$$. Thus any element of $$S(\bm{XA})$$ must be an element
of $$SX$$. Any element of $$S(X)$$ is also an element of
$$S(\bm{XA})$$. So these two subspaces must be identical. As a result, the
orthogonal projections $$\bm{P_X}$$ and $$\bm{P_{XA}}$$ should be same.

$$\begin{eqnarray}
\bm{P_{XA}}&=&\bm{XA}\left(\bm{A}^{T}X^{T}\bm{XA}\right)^{-1}\bm{A}^{T}X^{T}\\
&=&\bm{XA}\bm{A}^{-1}(X^{T}X)^{-1}(\bm{A}^{T})^{-1}\bm{A}^{T}X^{T}\\
&=&X(X^{T}X)^{-1}X^{T}=\bm{P_{X}}
\end{eqnarray}$$

We have known that the vectors of fitted values and residuals depend on
$$X$$ only through $$\bm{P_{X}}$$ and $$\bm{M_{X}}$$. Therefore, they too
must be invariant to any nonsingular linear transformation of the
columns of $$X$$.

If we replace $$X$$ by $$\bm{XA}$$ in the regression
$$y=\bm{X\beta}+u$$, the residuals and fitted values will not
change, even though $$\bm{\hat{\beta}}$$ will change.

# The Frisch-Waugh-Lovell Theorem

Consider the following two regressions 

$$\begin{eqnarray}
\label{eq20}
y&=&X_{1}\beta_{1}+X_{2}\beta_{2}+u\\
\label{eq21}
\bm{M}_{1}y&=&\bm{M}_{1}X_{2}\beta_{2}+\bm{M}_{1}u
\end{eqnarray}$$

::: proposition
Frisch-Waugh-Lovell Theorem

1.  The OLS estimates of $$\beta_{2}$$ from regressions
    (\ref{eq20}) and
    (\ref{eq21}) are
    numerically identical.

2.  The residuals from regressions
    (\ref{eq20}) and
    (\ref{eq21}) are
    numerically identical.
:::

Let $$\hat{\beta_{2}}$$ be the estimates of regression
(\ref{eq20}) and
$$\widetilde{\beta_{2}}$$ be the estimates of regression
(\ref{eq21})

::: proof
*Proof.* We define $$\hat{\be_{2}}$$ is the OLS estimator for $$\be_{2}$$ in
([\[eqfwl1\]](#eqfwl1){reference-type="ref" reference="eqfwl1"}) and
$$\tilde{\be_{2}}$$ is the OLS estimator for $$\be_{2}$$ in
([\[eqfwl2\]](#eqfwl2){reference-type="ref" reference="eqfwl2"}). We let
$$\hat{\bu}$$ be the residual for
([\[eqfwl1\]](#eqfwl1){reference-type="ref" reference="eqfwl1"}) and
$$\tilde{\bu}$$ for ([\[eqfwl2\]](#eqfwl2){reference-type="ref"
reference="eqfwl2"}).

First we prove result 1. 

$$\begin{eqnarray}
\tilde{\be_{2}}&=&\left((\m_{1}\x_{2})^{T}\m_{1}\x_{2}\right)^{-1}(\m_{1}\x_{2})^{T}\m_{1}\y\\
&=&\left(\x_{2}^{T}\m_{1}\x_{2}\right)^{-1}\x_{2}^{T}\m_{1}\y\\
&=&\left(\x_{2}^{T}\m_{1}\x_{2}\right)^{-1}\x_{2}^{T}\m_{1}(\x_{1}\hat{\be_{1}}+\x_{2}\hat{\be_{2}}+\m_{\x}\y)\\
&=&\left(\x_{2}^{T}\m_{1}\x_{2}\right)^{-1}\x_{2}^{T}\m_{1}\x_{2}\hat{\be_{2}}+\x_{2}^{T}\m_{1}\m_{\x}\y\\
&=&\left(\x_{2}^{T}\m_{1}\x_{2}\right)^{-1}\x_{2}^{T}\m_{1}\x_{2}\hat{\be_{2}}+\x_{2}^{T}\m_{\x}\y\\
&=&\left(\x_{2}^{T}\m_{1}\x_{2}\right)^{-1}\x_{2}^{T}\m_{1}\x_{2}\hat{\be_{2}}+(\m_{\x}\x_{2})^{T}\y\\
&=&\hat{\be_{2}}
\end{eqnarray}$$ Then we prove result 2 

$$\begin{eqnarray}
\m_{1}\y&=&\m_{1}(\x_{1}\hat{\be_{1}}+\x_{2}\hat{\be_{2}}+\m_{\x}\y)\\
&=&\m_{1}\x_{2}\hat{\be_{2}}+\m_{\x}\y\\
&=&\m_{1}\x_{2}\tilde{\be_{2}}+\m_{\x}\y\\
&=&\m_{1}\x_{2}\tilde{\be_{2}}+\hat{\bu}\\
\end{eqnarray}$$ We know $$\m_{1}\y=\m_{1}\x_{2}\tilde{\be_{2}}+\tilde{u}$$

Thus we have $$\tilde{\bu}=\hat{\bu}$$ ◻
:::

# Applications of FWL Theorem

## Goodness of Fit of a Regression

$$\begin{eqnarray}
TSS=\norm{y}^{2}&=&\norm{\bm{P_{X}y}}^{2}+\norm{\bm{M_{X}y}}^{2}=ESS+SSR
\end{eqnarray}$$

And we can define the **goodness of fit** for a regression model. The
measure is referred to as the $$\bm{R}^{2}$$ 

$$\begin{eqnarray}
\label{eqfwl3}
R^{2}_{u}&=&\frac{ESS}{TSS}=\frac{\norm{\bm{P_{X}y}}^{2}}{\norm{y}^{2}}=1-\frac{\norm{\bm{M_{X}y}}^{2}}{\norm{y}^{2}}=1-\frac{SSR}{TSS}=\cos \theta ^{2}
\end{eqnarray}$$

The $$R^{2}$$ defined in ([\[eqfwl3\]](#eqfwl3){reference-type="ref"
reference="eqfwl3"}) is called the **uncentered** $$\bm{R}^{2}$$. It is
invariant under nonsingular linear transformations of the regressors,
e.g. the changes in the scale of $$\y$$ (the angle $$\theta$$ remains same).
However, it will change when the changes of units change the angle
$$\theta$$.

We define the **centered** $$\bm{R}^{2}$$ 

$$\begin{eqnarray}
\label{eqfwl4}
R^{2}_{c}&=&\frac{\norm{\bm{P_{X}\m_{\iota}y}}^{2}}{\norm{\bm{\m_{\iota}y}}^{2}}=1-\frac{\norm{\bm{M_{X}y}}^{2}}{\norm{\bm{\m_{\iota}y}}^{2}}
\end{eqnarray}$$

# Influential Observations and Leverage

One or a few observations in a regression are highly **influential**, in
the sense that deleting them from the sample would change some elements
of $$\hat{\be}$$ substantially.

## Leverage

The effect of a single observation on $$\hat{\be}$$ can be seen by
comparing $$\hat{\be}$$ with $$\hat{\be}^{t}$$, the estimate of $$\be$$ that
would be obtained if the $$t^{th}$$ observation were omitted from the
sample.

Let $$\bm{e}_{t}=\left[\begin{array}{ccccccc}
0&\cdots&0 &1&0&\cdots&0
\end{array}\right]^{T}$$ is n $$n$$-vector which has $$t^{th}$$ element 1 and
all other element 0. Including $$\e$$ as a regressor 

$$\begin{eqnarray}
\label{eq22}
\y&=&\x\be+\alpha \e+\bu
\end{eqnarray}$$ 

By FWL, 

$$\begin{eqnarray}
\label{eq23}
\m_{t}\y&=&\m_{t}\x\be+\mbox{residuals}
\end{eqnarray}$$ 

where $$\m_{t}=\m_{\e}=\bm{I}-\e(\e^{T}\e)^{-1}\e^{T}$$.
It is easy to find 

$$\begin{eqnarray}
\m_{t}\y&=&\y-\e(\e^{T}\e)^{-1}\e^{T}\y=\y-\e\e^{T}\y=\y-y_{t}\e
\end{eqnarray}$$ 

Thus $$y_{t}$$ is subtracted from $$\y$$ fro the $$t^{th}$$
observation only. Similarly, $$\m_{t}\x$$ is just $$\x$$ with its $$t^{th}$$
row replaced by zeros. Therefore, **running
([\[eq23\]](#eq23){reference-type="ref" reference="eq23"}) will give the
same parameter estimates as those that would be obtained if we deleted
observation $$t$$ from the sample.**

Let $$\p_{\z}$$ and $$\m_{\z}$$ be the orthogonal projections on to and off
$$S(\x,\e)$$. 

$$\begin{eqnarray}
\label{eq24}
\y&=&\p_{\z}\y+\m_{\z}\y=\x\hat{\be}^{t}+\hat{\alpha}\e+\m_{\z}\y
\end{eqnarray}$$ 

Premultiply by $$\p_{\x}$$ 

$$\begin{eqnarray}
\p_{\x}\y&=&\x\hat{\be}^{t}+\hat{\alpha}\p_{\x}\e
\end{eqnarray}$$ 

So we have 

$$\begin{eqnarray}
\x\hat{\be}&=&\x\hat{\be}^{t}+\hat{\alpha}\p_{\x}\e\\
\x(\hat{\be}^{t}-\hat{\be})&=&-\hat{\alpha}\p_{\x}\e
\end{eqnarray}$$

Now we need to calculate $$\hat{\alpha}$$. By FWL, from
([\[eq22\]](#eq22){reference-type="ref" reference="eq22"}) we get

$$\begin{eqnarray}
\m_{\x}\y&=&\hat{\alpha}\m_{\x}\e+\mbox{residuals}
\end{eqnarray}$$ 

and we have 

$$\begin{eqnarray}
\hat{\alpha}&=&((\m_{\x}\e)^{T}\m_{\x}\e)^{-1}(\m_{\x}\e)^{T}\m_{\x}\y\\
&=&\frac{\e^{T}\m_{\x}\y}{\e^{T}\m_{\x}\e}
\end{eqnarray}$$ 

where $$\e^{T}\m_{\x}\y$$ is the $$t^{th}$$ element of
$$\m_{\x}\y$$ and we denote this element as $$\hat{u}_{t}$$. Similarly,
$$\e^{T}\m_{\x}\e$$ is the $$t^{th}$$ diagonal element of $$\m_{\x}$$. So we
have 

$$\begin{eqnarray}
\label{eq25}
\hat{\alpha}&=&\frac{\hat{u}_{t}}{1-h_{t}}
\end{eqnarray}$$ where $$h_{t}$$ is the $$t^{th}$$ diagonal element of
$$\p_{\x}$$.

So we have 

$$\begin{eqnarray}
\x(\hat{\be}^{t}-\hat{\be})&=&-\hat{\alpha}\p_{\x}\e\\
(\x^{T}\x)^{-1}\x^{T}\x(\hat{\be}^{t}-\hat{\be})&=&-\frac{\hat{u}_{t}}{1-h_{t}}(\x^{T}\x)^{-1}\x^{T}\p_{\x}\e\\
\hat{\be}^{t}-\hat{\be}&=&-\frac{\hat{u}_{t}}{1-h_{t}}(\x^{T}\x)^{-1}\x^{T}\p_{\x}\e\\
&=&-\frac{\hat{u}_{t}}{1-h_{t}}(\x^{T}\x)^{-1}\x^{T}_{t}\hat{u}_{t}
\end{eqnarray}$$